Composite literal for slices

new/golang/defn/slice.v
@@ -22,24 +22,10 @@ Definition for_range (elem_type : go.type) : val :=
                       (λ: <>, "i" <-[go.int] (![go.int] "i") + #(W64 1)) :=
     (λ: <>, "body" (![go.int] "i") (![elem_type] (IndexRef (go.SliceType elem_type)) ("s", (![go.int] "i")))).
 
-(* Takes in a list as input, and turns it into a heap-allocated slice. *)
-Definition literal (elem_type : go.type) : val :=
-  λ: "elems",
-  let st : go.type := go.SliceType elem_type in
-  let: "len" := ArrayLength "elems" in
-  let: "s" := FuncResolve go.make2 [st] #() "len" in
-  let: "l" := ref "elems" in
-  let: "i" := GoAlloc go.int #() in
-  (for: (λ: <>, (![go.int] "i") <⟨go.int⟩ "len") ; (λ: <>, "i" <-[go.int] ![go.int] "i" + #(W64 1)) :=
-     (λ: <>,
-        do: (IndexRef st ("s", (![go.int] "i")) <-[elem_type]
-                (Index (go.ArrayType (2^63) elem_type) ("elems", ![go.int] "i"))))) ;;
-  "s".
-
 End goose_lang.
 End slice.
 
-Global Opaque slice.for_range slice.literal.
+Global Opaque slice.for_range.
 
 Module go.
 Class SliceSemantics {ext : ffi_syntax} `{!GoContext} :=
@@ -121,6 +107,16 @@ Class SliceSemantics {ext : ffi_syntax} `{!GoContext} :=
          FuncResolve go.copy [st] #() "s_new" "s" ;;
          FuncResolve go.copy [st] #() (Slice st ("s_new", (FuncResolve go.len [st] #() "s", "new_len"))) "x" ;;
          "s_new")%V;
+
+  composite_literal_slice elem_type (vs : list val) :
+    composite_literal (go.SliceType elem_type) (ArrayV vs) =
+    if decide (Z.of_nat (length vs) < 2^63) then
+      (let: "tmp" := GoAlloc (go.ArrayType (length vs) elem_type) #() in
+       "tmp" <-[(go.ArrayType (length vs) elem_type)]
+                CompositeLiteral (go.ArrayType (length vs) elem_type) (ArrayV vs);;
+       Slice (go.ArrayType (length vs) elem_type) ("tmp", (#(W64 0), #(W64 (length vs))))
+      )%E
+    else AngelicExit #();
 
   array_index_ref_0 t l : array_index_ref t 0 l = l;
 }.
